Axioms.v
@@ -1,0 +1,126 @@
+Require Import Coq.Sets.Constructive_sets.
+Require Import Definitions.
+Require Import Operational_Semantics.
+Require Import Contracts_Subst.
+
+
+
+
+
+
+
+(*---Well-Formedness of Executions *)
+Axiom FW: forall (Ex:Exec), (WF1 Ex) ->(WF2 Ex) ->(WF3 Ex) ->(WF4 Ex) ->(WF5 Ex) ->(WF6 Ex)-> (WF7 Ex) ->(WF Ex). 
+Axiom WFhelp: forall (Ex:Exec), (WF Ex)->(WF1 Ex)/\(WF2 Ex)/\(WF3 Ex)/\(WF4 Ex)/\(WF5 Ex)/\(WF6 Ex)/\(WF7 Ex).
+
+
+
+(*---Freshness of the Newly Generated Effect *)
+Axiom Freshness: forall (Θ:Store)(ex1 ex2:Exec) (opk:op_key)(eff:Effect)(r:ReplID),  
+                   [Θ|-ex1, opk ~r~> ex2, eff] -> forall r, (dom Θ r)-> ~ (Θ r) eff.
+Axiom CorrectFreshness: forall(Θ:Store)(ex1 ex2:Exec)(opk:op_key)(eff:Effect)(r:ReplID), 
+                          [Θ|-ex1, opk ~r~> ex2, eff] -> ~ (ex1-A) eff.
+
+
+(*---The Definition of Equality of two Session Soups *)
+Axiom  Sess_Equal : forall (S S':SessSoup), S=S' <-> forall (I:Soup_Ing), (In Soup_Ing S I <-> In Soup_Ing S' I).
+
+
+(*---Trivial Facts About Relations*)
+Axiom sameobj_trans: forall (Ex:Exec)(a b c: Effect), Ex-sameobj a b -> Ex-sameobj b c -> Ex-sameobj a c.
+Axiom Sameobj_Def: forall  (Θ:Store) (Ex Ex':Exec)(opk:op_key) (η:Effect) (r:ReplID) (a b: Effect),
+                     [Θ |- Ex, opk ~r~> Ex', η] -> Ex-A a -> Ex-A b -> Ex-sameobj a b.
+Axiom SO_Seq_General : forall (Ex:Exec) (a b:Effect), (Ex-so a b) <-> (lt (seq a) (seq b)). 
+
+
+
+(*---Relating Domain of the Relations to the Universe of Effects*)
+Axiom So_Domain :      forall (Ex:Exec)(a:Effect), ((Rel_dom Ex-so a)      -> (Ex-A a)).
+Axiom Vis_Domain :     forall (Ex:Exec)(a:Effect), ((Rel_dom Ex-vis a)     -> (Ex-A a)).
+Axiom Hbo_Domain :     forall (Ex:Exec)(a:Effect), ((Rel_dom Ex-hbo a)     -> (Ex-A a)).
+Axiom Sameobj_Domain : forall (Ex:Exec)(a:Effect), ((Rel_dom Ex-sameobj a) -> (Ex-A a)).
+
+(*---The Conclusion from Equality of Soup Ingredients*)
+Axiom Seq_Uniq : forall (i i': SeqNo)(s s': SessID)(σ σ' : session), (<<s , i , σ >>) = (<<s', i' , σ' >>) -> i=i'.
+
+
+(*--- So only relates effects from the same session*)
+Axiom SO_SameSession : forall (Ex:Exec)(eff eff':Effect), Ex-so eff eff' -> (eff.(sess) = eff'.(sess)).
+
+(*---Decidability of Membership of a Soup *)
+Axiom Soup_comp : forall (Ex:Exec)(eff:Effect), (Ex-A eff)\/(~ Ex-A eff).
+
+
+(*---Claimed in the Paper *)
+(*3 equal statements to the acyclicity of hb*)
+Axiom PaperH8: forall (Ex:Exec)(eff:Effect), ~ (Ex-hb eff eff)-> ((~Ex-vis eff eff) /\ (~ Ex-so eff eff)).
+
+Axiom PaperH8II : forall (Ex:Exec)(eff eff': Effect), ~((Ex-vis eff eff')/\ (Ex-so eff' eff)).
+
+Axiom PaperH8III : forall (Ex:Exec), 
+                     (forall (eff:Effect), Ex-A eff -> ~ Ex-vis eff eff) ->
+                     (forall (eff:Effect), Ex-A eff -> ~ Ex-so  eff eff) ->
+                     (forall (eff eff':Effect),Ex-A eff -> Ex-A eff' ->  ~((Ex-vis eff eff')/\ (Ex-so eff' eff))) ->
+                     (forall (eff:Effect),~(Ex-hb eff eff)).
+
+
+(*---Equality if Effect Variables is Reflexive*)
+Axiom  Eff_Equi_refl : forall a,  Eff_Equi a a.
+
+(*---Relating Error term, to the domain of the Stores*)
+Axiom error_not_domain: forall (r:ReplID)(t:Store),  (t r = St_Dom_Error) <-> (~(dom t) r).
+
+(*---Equaility of ReplIDs is decidable*)
+Axiom ReplID_Equality_Decidable: forall (r r':ReplID), (r=r') \/ (r<>r').
+
+
+
+(*************************************************************************************************************************)
+(*=============================These Were Axioms Before, But Now Are Replaced with Other Axioms and Are Trivially Proved *)
+
+Lemma  SO_NewEff: forall (Θ: Store)(Ex Ex':Exec) (opk:op_key)(η:Effect)(r:ReplID),
+                    [Θ|-Ex, opk ~r~> Ex', η] -> (forall a:Effect, Θ r a -> ~ Ex-so η a).
+Proof. intuition. apply CorrectFreshness in H. apply WF_Relation with (a:= η) (b:=a) in H1; destruct H1.
+       apply So_Domain in H1; auto.
+Qed.
+
+Require Import Omega.
+
+Lemma SessionOrder : forall (Ex:Exec)(eff eff':Effect), Ex-so eff eff' -> ((eff.(sess) = eff'.(sess))/\ ((eff.(seq))+1 <= (eff'.(seq)))).
+Proof.
+  intros Ex a b Hso. split.
+  apply SO_SameSession in Hso; auto. apply SO_Seq_General in Hso. intuition.
+Qed.
+
+Lemma  SO_Seq : forall (Ex:Exec)(a b c:Effect), Ex-so a b -> seq b = seq c - 1 -> Ex-so a c.
+Proof.
+  intros Ex a b c. intros Hso Heq. apply SO_Seq_General. apply SO_Seq_General in Hso. intuition.
+Qed.
+
+Lemma SO_SeqII' : forall (Ex:Exec)(a b :Effect), (seq b>0)->seq a = seq b -1  -> Ex-so a b.
+Proof.
+  intros. apply SO_Seq_General. omega.
+Qed.
+
+Lemma Eneq_nat_cont : forall i:SeqNo, (i>0)->(i=i-1)\/(i=i+1) -> False.
+Proof. intros. omega.
+Qed.
+
+Lemma natSeq: forall ss:SeqNo, ~(ss+1 <= (ss-1)).
+Proof.
+  intros. omega.
+Qed.
+
+Lemma  SO_SeqIII : forall (Ex:Exec)(a b c:Effect), Ex-so a b -> Ex-so b c  -> Ex-so a c.
+Proof.
+  intros.
+  apply SO_Seq_General. apply SO_Seq_General in H. apply SO_Seq_General in H0. omega.
+Qed.
+
+
+Lemma Relation_Dom : forall (Ex:Exec) (eff:Effect), (~Ex-A eff ) -> (~Ex-so eff eff).
+  Proof.
+    intuition. apply WF_Relation with (a:=eff)(b:=eff)(r:=Ex-so) in H0. destruct H0.
+    apply So_Domain in H1; auto.
+Qed.
+
