Contracts_Definition.v
@@ -1,0 +1,89 @@
+Require Import Coq.Strings.String.
+Require Import Definitions.
+
+Parameter Eff_name : Effect -> string.
+
+Inductive EffVar : Type :=
+|effvar: string -> EffVar.
+
+Definition η'':=effvar "η''".
+
+
+Inductive contract_EffType : Type :=
+|contract_EffType_cons: OperName -> contract_EffType
+|contract_efftype_disjunction: contract_EffType -> contract_EffType -> contract_EffType.
+
+Inductive contract_Relation : Type :=
+|contract_equi: contract_Relation
+|contract_vis: contract_Relation
+|contract_so: contract_Relation
+|contract_sameobj: contract_Relation
+|contract_relation_union: contract_Relation -> contract_Relation -> contract_Relation
+|contract_relation_intersect: contract_Relation -> contract_Relation -> contract_Relation
+|contract_relation_closure: contract_Relation -> contract_Relation.
+
+Definition Soo : contract_Relation :=
+  contract_relation_intersect contract_so contract_sameobj.
+
+Definition Hb : contract_Relation :=
+  contract_relation_closure (contract_relation_union contract_so contract_vis).
+
+Definition Hbo:contract_Relation :=
+  contract_relation_closure(contract_relation_union Soo contract_vis).
+
+Inductive contract_Prop : Type :=
+|contract_prop_true
+|contract_prop_effeff : contract_Relation -> Effect -> Effect -> contract_Prop
+|contract_prop_effvar : contract_Relation -> Effect -> EffVar -> contract_Prop
+|contract_prop_vareff : contract_Relation -> EffVar -> Effect -> contract_Prop
+|contract_prop_varvar : contract_Relation -> EffVar -> EffVar -> contract_Prop                                     
+|contract_prop_disjunction: contract_Prop -> contract_Prop   -> contract_Prop
+|contract_prop_conjunction: contract_Prop -> contract_Prop   -> contract_Prop
+|contract_prop_implication: contract_Prop -> contract_Prop   -> contract_Prop.      
+
+Inductive contract_Contract : Type :=
+|contract_free_cons: contract_Prop -> contract_Contract
+|contract_untyped_cons: EffVar->contract_Contract -> contract_Contract
+|contract_typed_cons: EffVar -> contract_EffType -> contract_Contract -> contract_Contract.
+
+
+
+
+Definition m:EffVar := effvar "m".
+Definition n:EffVar :=effvar "n".
+Infix " '#-->' " := contract_prop_implication (at level 80).
+Infix " '#\/#' " := contract_prop_disjunction (at level 70).
+Infix " '#/\#' " := contract_prop_conjunction (at level 60).
+Notation " 'Sameobj' " := contract_sameobj.
+Notation " 'Vis' " := contract_vis.
+Notation " 'Equi' " := contract_equi.
+Notation " 'PROP:'  ":= contract_prop_varvar (at level 90).
+Notation " 'CONTR:'  ":=contract_free_cons (at level 95).
+Notation " 'ALL'  ":=(contract_untyped_cons) (at level 96).
+
+
+
+(*================================ Store Consistency *)
+
+Definition Store_Contr (τ:ConsCls):contract_Contract:=
+  match τ with
+    |sc =>ALL  m (CONTR: ((PROP: Sameobj m η'')   #-->
+                                                 ((PROP: Vis m η'') #\/# (PROP: Vis η'' m) #\/#
+                                                                    (PROP: Equi m η''))))
+    |cc => ALL m (CONTR: ((PROP: Hbo m η'') #--> (PROP: Vis m η'')))
+    |ec => ALL m (ALL n (CONTR: ((PROP: Hbo m n) #/\# (PROP: Vis n η'') #--> (PROP: Vis m η''))))
+  end.
+
+Notation " 'Ψ' " := Store_Contr.
+
+
+
+
+
+
+
+
+
+
+
+
