Contracts_Evaluation.v
@@ -1,0 +1,66 @@
+Require Import Definitions.
+Require Import Contracts_Subst.
+Require Import Coq.Strings.String.
+Require Import Contracts_Definition.
+
+
+
+Fixpoint relation_Evaluation (rel : contract_Relation) (Ex:Exec) : Relation :=
+  match rel with
+    |contract_equi => Eff_Equi
+    |contract_vis   => Ex-vis
+    |contract_so => Ex-so
+    |contract_sameobj => Ex-sameobj
+    |contract_relation_union R1 R2 => Rel_Union (relation_Evaluation R1 Ex) (relation_Evaluation R2 Ex)
+    |contract_relation_intersect R1 R2 => Rel_Intersect (relation_Evaluation R1 Ex)  (relation_Evaluation R2 Ex)
+    |contract_relation_closure R1 => (Rel_Closure  (relation_Evaluation R1 Ex))
+  end.
+
+Fixpoint Prop_Evaluation (pr:contract_Prop)(Ex:Exec) : Prop:=
+  match pr with
+    |contract_prop_true => True
+    |contract_prop_effeff R1 α β      => (relation_Evaluation R1 Ex) α β
+    |contract_prop_conjunction p1 p2  =>  (Prop_Evaluation p1 Ex) /\ (Prop_Evaluation p2 Ex)
+    |contract_prop_disjunction p1 p2  =>  (Prop_Evaluation p1 Ex) \/  (Prop_Evaluation p2 Ex)
+    |contract_prop_implication p1 p2  =>  (Prop_Evaluation p1 Ex) ->  (Prop_Evaluation p2 Ex)
+    |_=> False                                                          
+  end.
+
+Fixpoint contract_Eval (cont: contract_Contract) (Ex:Exec) (eff : Effect) (n:nat):Prop :=
+  match n with
+    |O => match cont with
+           |contract_free_cons π => Prop_Evaluation (Prop_Subst π eff η'') Ex
+           |_=> False
+         end
+          
+    |S n' => match cont with
+              |contract_typed_cons e τ ψ =>  forall ef:Effect,(Ex-A ef) -> contract_Eval (contract_Subst ψ ef e) Ex eff n'
+              |contract_untyped_cons e ψ =>  forall ef:Effect,(Ex-A ef) -> contract_Eval (contract_Subst ψ ef e) Ex eff n' 
+              |_=> False
+            end
+  end.
+
+                       
+Fixpoint contract_free_number (cont:contract_Contract) : nat :=
+  match cont with
+    |contract_free_cons p => 0
+    |contract_untyped_cons e ψ => contract_free_number ψ +1
+    |contract_typed_cons e t ψ => contract_free_number ψ +1
+  end.
+
+
+
+
+
+
+
+
+
+
+
+
+
+
+
+
+
