Theorem8_Lemmas.v
@@ -1,41 +1,28 @@
-Require Import case_coq.
-Require Import List.
+Require Import Cases.
 Require Import Coq.Sets.Constructive_sets.
-Require Import Coq.Arith.EqNat.
-Require Import Coq.Relations.Relation_Definitions.
-Require Import Coq.Relations.Relation_Operators.
-Require Import Coq.Arith.Compare_dec.
-Require Import Coq.Program.Tactics.
 Require Import Definitions.
-Require Import oper_semantic_coq.
-Require Import axioms_coq.
-Require Import theorems_coq.
-Require Import contract_definition.
-Require Import contract_subs.
-Require Import contract_Eval.
-Require Import lemma5.
-Require Import Theorem7_Lemma.
-Require Import Theorem7.
+Require Import Axioms.
 Require Import Omega.
-Import Operational_Semantics.
 
-
+(*----------------------------------------------------*)
+(*Trivial Assertion About Binders of Replica IDs*)
 Lemma rid_same_binder: forall (r:ReplID), (beq_nat (Rid_to_nat r)(Rid_to_nat r)) = true.
 Proof.
-  intro r.
-  induction r. simpl. induction n.
+  intro r. induction r. simpl. induction n.
   reflexivity. simpl. apply IHn.
 Qed.
 
-  
+
+(*----------------------------------------------------*)
 Lemma  Theorem8_beq_help:  forall η θ r,  F_Union θ r η r = Union Effect ( θ r) (Singleton Effect η).
 Proof. intros. unfold F_Union.
-         rewrite rid_same_binder. reflexivity.
+       rewrite rid_same_binder. reflexivity.
 Qed.
 
-Axiom error_not_domain: forall (r:ReplID)(t:Store),  (t r = St_Dom_Error) <-> (~(dom t) r).
-Axiom ReplID_Equality_Decidable: forall (r r':ReplID), (r=r') \/ (r<>r').
 
+
+(*----------------------------------------------------*)
+(*Two ReplIDs are the same, iff their binders are the same number*)
 Lemma Theorem8_dom_help'_help: forall r r', r=r' <->  (beq_nat (Rid_to_nat r) (Rid_to_nat r')=true).
 Proof.
   intros r r'.
@@ -48,19 +35,23 @@ Proof.
 Qed.   
 
 
-                                 
+
+(*----------------------------------------------------*)
+(*F_Union of something, has only one element in its domain!*)
 Lemma Theorem8_dom_help' : forall η θ r' r,  dom (F_Union θ r η) r' -> r'=r.
 Proof.
-intros. 
-assert (r=r' \/ r<>r') as HRidDec; try( apply ReplID_Equality_Decidable).
-destruct HRidDec; auto. apply error_not_domain in H; intuition. 
-destruct (beq_nat (Rid_to_nat r) (Rid_to_nat r')) eqn:E. compute. apply Theorem8_dom_help'_help in E; intuition.
-unfold F_Union. rewrite E. reflexivity.
+  intros. 
+  assert (r=r' \/ r<>r') as HRidDec; try( apply ReplID_Equality_Decidable).
+  destruct HRidDec; auto. apply error_not_domain in H; intuition. 
+  destruct (beq_nat (Rid_to_nat r) (Rid_to_nat r')) eqn:E. compute. apply Theorem8_dom_help'_help in E; intuition.
+  unfold F_Union. rewrite E. reflexivity.
 Qed.
 
 
-  
 
+
+(*----------------------------------------------------*)
+(*forall i>0, i-1 is less than i*)
 Lemma Theorem8_nat_help : forall i:SeqNo, (i<>0) -> (lt (i-1) i).
 Proof.
   intros.
